EvmSmith.lean
@@ -17,6 +17,7 @@ import EvmSmith.Demos.Weth.Solvency
 import EvmSmith.Demos.Weth.EntryPoints
 import EvmSmith.Demos.Weth.Dispatch
 import EvmSmith.Demos.Weth.Behaviour
+import EvmSmith.Demos.Weth.SpecDSL
 import EvmSmith.Demos.Weth.Spec
 import EvmSmith.Demos.Weth.OptimizedProgram
 import EvmSmith.Demos.Tests
